src/lean4/human_eval/problem_91.lean
@@ -1,0 +1,83 @@
+import Imports.AllImports
+
+-- start_def problem_details
+/--
+function_signature: "def is_bored(s: str) -> int"
+docstring: |
+    You'll be given a string of words, and your task is to count the number
+    of boredoms. A boredom is a sentence that starts with the word "I".
+    Sentences are delimited by '.', '?' or '!'.
+test_cases:
+  - input: "Hello world"
+    expected_output: 0
+  - input: "The sky is blue. The sun is shining. I love this weather"
+    expected_output: 1
+-/
+-- end_def problem_details
+
+-- start_def problem_spec
+def problem_spec
+-- function signature
+(implementation: String → Nat)
+-- inputs
+(s: String) :=
+-- spec
+let spec (result : Nat) :=
+  let is_sentence_is_boredom (s: String) : Bool :=
+    (s.startsWith "I " ∨ s.startsWith " I") ∧ '.' ∉ s.data ∧ '?' ∉ s.data ∧ '!' ∉ s.data
+  match s.data.findIdx? (λ c => c = '.' ∨ c = '?' ∨ c = '!') with
+  | some i =>
+    let j := i + 1;
+    let substring := s.drop j;
+    result = (if is_sentence_is_boredom substring then 1 else 0) + implementation substring
+  | none =>
+    result = if is_sentence_is_boredom s then 1 else 0
+-- program termination
+∃ result,
+  implementation s = result ∧
+  spec result
+-- end_def problem_spec
+
+-- start_def generated_spec
+def generated_spec
+-- function signature
+(impl: String → Nat)
+-- inputs
+(s: String) : Prop :=
+--end_def generated_spec
+--start_def generated_spec_body
+sorry
+--end_def generated_spec_body
+
+-- start_def spec_isomorphism
+theorem spec_isomorphism:
+∀ impl,
+(∀ s, problem_spec impl s) ↔
+(∀ s, generated_spec impl s) :=
+-- end_def spec_isomorphism
+-- start_def spec_isomorphism_proof
+sorry
+-- end_def spec_isomorphism_proof
+
+-- start_def implementation_signature
+def implementation (s: String) : Nat := sorry
+-- end_def implementation_signature
+
+-- start_def implementation
+-- end_def implementation
+
+-- start_def test_cases
+-- #test implementation "Hello world" = 0
+-- #test implementation "The sky is blue. The sun is shining. I love this weather" = 1
+-- end_def test_cases
+
+-- start_def correctness_definition
+theorem correctness
+(s: String)
+: problem_spec implementation s
+:=
+-- end_def correctness_definition
+-- start_def correctness_proof
+by
+sorry
+-- end_def correctness_proof
