src/lean4/human_eval/problem_94.lean
@@ -1,0 +1,91 @@
+import Imports.AllImports
+
+-- start_def problem_details
+/--
+function_signature: "def skjkasdkd(lst : list[int]) -> int"
+docstring: |
+    You are given a list of integers.
+    You need to find the largest prime value and return the sum of its digits.
+test_cases:
+  - input: [0,3,2,1,3,5,7,4,5,5,5,2,181,32,4,32,3,2,32,324,4,3]
+    expected_output: 10
+  - input: [1,0,1,8,2,4597,2,1,3,40,1,2,1,2,4,2,5,1]
+    expected_output: 25
+  - input: [1,3,1,32,5107,34,83278,109,163,23,2323,32,30,1,9,3]
+    expected_output: 13
+  - input: [0,724,32,71,99,32,6,0,5,91,83,0,5,6]
+    expected_output: 11
+  - input: [0,81,12,3,1,21]
+    expected_output: 3
+  - input: [0,8,1,2,1,7]
+    expected_output: 7
+-/
+-- end_def problem_details
+
+-- start_def problem_spec
+def problem_spec
+-- function signature
+(implementation: List Int → Int)
+-- inputs
+(lst: List Int) :=
+-- spec
+let spec (result : Int) :=
+  match result with
+  | 0 => ¬ (∃ i, i < lst.length ∧ Prime (lst.get! i))
+  | _ => result > 0 ∧ ∃ i, i < lst.length ∧ Prime (lst.get! i) ∧
+    (∀ j, j < lst.length ∧ Prime (lst.get! j) → lst.get! i ≤ lst.get! j) ∧
+    result = (Nat.digits 10 (lst.get! i).toNat).sum
+-- program termination
+∃ result,
+  implementation lst = result ∧
+  spec result
+
+-- start_def generated_spec
+def generated_spec
+-- function signature
+(impl: List Int → Int)
+-- inputs
+(lst: List Int) : Prop :=
+--end_def generated_spec
+--start_def generated_spec_body
+sorry
+--end_def generated_spec_body
+
+-- start_def spec_isomorphism
+theorem spec_isomorphism:
+∀ impl,
+(∀ lst, problem_spec impl lst) ↔
+(∀ lst, generated_spec impl lst) :=
+-- end_def spec_isomorphism
+-- start_def spec_isomorphism_proof
+sorry
+-- end_def spec_isomorphism_proof
+
+
+-- start_def implementation_signature
+def implementation (lst: List Int) : Int := sorry
+-- end_def implementation_signature
+
+-- start_def implementation
+-- end_def implementation
+
+-- start_def test_cases
+-- #test implementation [0,3,2,1,3,5,7,4,5,5,5,2,181,32,4,32,3,2,32,324,4,3] = 10
+-- #test implementation [1,0,1,8,2,4597,2,1,3,40,1,2,1,2,4,2,5,1] = 25
+-- #test implementation [1,3,1,32,5107,34,83278,109,163,23,2323,32,30,1,9,3] = 13
+-- #test implementation [0,724,32,71,99,32,6,0,5,91,83,0,5,6] = 11
+-- #test implementation [0,81,12,3,1,21] = 3
+-- #test implementation [0,8,1,2,1,7] = 7
+-- end_def test_cases
+
+
+-- start_def correctness_definition
+theorem correctness
+(lst: List Int)
+: problem_spec implementation lst
+:=
+-- end_def correctness_definition
+-- start_def correctness_proof
+by
+sorry
+-- end_def correctness_proof
