src/lean4/human_eval/problem_96.lean
@@ -1,0 +1,90 @@
+import Imports.AllImports
+
+-- start_def problem_details
+/--
+function_signature: "def count_up_to(n : Int) -> List Int"
+docstring: |
+    Implement a function that takes an non-negative integer and returns an array of the first n
+    integers that are prime numbers and less than n.
+test_cases:
+  - input: 5
+    expected_output: [2,3]
+  - input: 11
+    expected_output: [2,3,5,7]
+  - input: 0
+    expected_output: []
+  - input: 20
+    expected_output: [2,3,5,7,11,13,17,19]
+  - input: 1
+    expected_output: []
+  - input: 18
+    expected_output: [2,3,5,7,11,13,17]
+-/
+-- end_def problem_details
+
+-- start_def problem_spec
+def problem_spec
+-- function signature
+(implementation: Int → List Int)
+-- inputs
+(n: Int) :=
+-- spec
+let spec (result : List Int) :=
+  match n with
+  | 0 => result = []
+  | n => n > 0 → (∀ i, i < result.length → (Nat.Prime (result.get! i).toNat) ∧ (result.get! i) < n) ∧
+         (∀ i : Nat, i < n → Nat.Prime i → (i : ℤ) ∈ result)
+-- program termination
+∃ result,
+  implementation n = result ∧
+  spec result
+
+-- start_def generated_spec
+def generated_spec
+-- function signature
+(impl: Int → List Int)
+-- inputs
+(n: Int) : Prop :=
+--end_def generated_spec
+--start_def generated_spec_body
+sorry
+--end_def generated_spec_body
+
+-- start_def spec_isomorphism
+theorem spec_isomorphism:
+∀ impl,
+(∀ n, problem_spec impl n) ↔
+(∀ n, generated_spec impl n) :=
+-- end_def spec_isomorphism
+-- start_def spec_isomorphism_proof
+sorry
+-- end_def spec_isomorphism_proof
+
+
+-- start_def implementation_signature
+def implementation (n: Int) : List Int := sorry
+-- end_def implementation_signature
+
+-- start_def implementation
+-- end_def implementation
+
+-- start_def test_cases
+-- #test implementation 5 = [2,3]
+-- #test implementation 11 = [2,3,5,7]
+-- #test implementation 0 = []
+-- #test implementation 20 = [2,3,5,7,11,13,17,19]
+-- #test implementation 1 = []
+-- #test implementation 18 = [2,3,5,7,11,13,17]
+-- end_def test_cases
+
+
+-- start_def correctness_definition
+theorem correctness
+(n: Int)
+: problem_spec implementation n
+:=
+-- end_def correctness_definition
+-- start_def correctness_proof
+by
+sorry
+-- end_def correctness_proof
