src/lean4/human_eval/problem_97.lean
@@ -1,0 +1,83 @@
+import Imports.AllImports
+
+-- start_def problem_details
+/--
+function_signature: "def multiply(a : Int, b : Int) -> Int"
+docstring: |
+    Complete the function that takes two integers and returns
+    the product of their unit digits.
+    Assume the input is always valid.
+    -- Note(George): I'm finding it hard to not leak the implementation here, so I opted to make the spec more convoluted.
+test_cases:
+  - input: 148, 412
+    expected_output: 16
+  - input: 19, 28
+    expected_output: 72
+  - input: 2020, 1851
+    expected_output: 0
+  - input: 14, -15
+    expected_output: 20
+-/
+-- end_def problem_details
+
+-- start_def problem_spec
+def problem_spec
+-- function signature
+(implementation: Int → Int → Int)
+-- inputs
+(a b: Int) :=
+-- spec
+let spec (result : Int) :=
+  result + (a % 10) * b + a * (b % 10) + (a - a % 10) * (b - b % 10) = a * b
+-- program termination
+∃ result,
+  implementation a b = result ∧
+  spec result
+
+-- start_def generated_spec
+def generated_spec
+-- function signature
+(impl: Int → Int → Int)
+-- inputs
+(a b: Int) : Prop :=
+--end_def generated_spec
+--start_def generated_spec_body
+sorry
+--end_def generated_spec_body
+
+-- start_def spec_isomorphism
+theorem spec_isomorphism:
+∀ impl,
+(∀ a b, problem_spec impl a b) ↔
+(∀ a b, generated_spec impl a b) :=
+-- end_def spec_isomorphism
+-- start_def spec_isomorphism_proof
+sorry
+-- end_def spec_isomorphism_proof
+
+
+-- start_def implementation_signature
+def implementation (a b: Int) : Int := sorry
+-- end_def implementation_signature
+
+-- start_def implementation
+-- end_def implementation
+
+-- start_def test_cases
+-- #test implementation 148 412 = 16
+-- #test implementation 19 28 = 72
+-- #test implementation 2020 1851 = 0
+-- #test implementation 14 -15 = 20
+-- end_def test_cases
+
+
+-- start_def correctness_definition
+theorem correctness
+(a b: Int)
+: problem_spec implementation a b
+:=
+-- end_def correctness_definition
+-- start_def correctness_proof
+by
+sorry
+-- end_def correctness_proof
