src/lean4/human_eval/problem_98.lean
@@ -1,0 +1,81 @@
+import Imports.AllImports
+
+-- start_def problem_details
+/--
+function_signature: "def count_upper(s : String) -> Int"
+docstring: |
+    Given a string s, count the number of uppercase vowels in even indices.
+    -- Note(George): I also feel like this one is hard to not leak, I tried a trick about keeping implementation for a recursive call in the spec. Let me know if this doesn't work..
+test_cases:
+  - input: "aBCdEf"
+    expected_output: 1
+  - input: "abcdefg"
+    expected_output: 0
+  - input: "dBBE"
+    expected_output: 0
+-/
+-- end_def problem_details
+
+-- start_def problem_spec
+def problem_spec
+-- function signature
+(implementation: String → Int)
+-- inputs
+(s: String) :=
+-- spec
+let uppercase_vowels := ["A", "E", "I", "O", "U"]
+let spec (result : Int) := match s.data with
+| [] => result = 0
+| _ :: [] => result = 0
+| c :: _ :: cs => result = (if uppercase_vowels.contains (String.mk [c]) then 1 else 0) + implementation (String.mk cs)
+-- program termination
+∃ result,
+  implementation s = result ∧
+  spec result
+
+-- start_def generated_spec
+def generated_spec
+-- function signature
+(impl: String → Int)
+-- inputs
+(s: String) : Prop :=
+--end_def generated_spec
+--start_def generated_spec_body
+sorry
+--end_def generated_spec_body
+
+-- start_def spec_isomorphism
+theorem spec_isomorphism:
+∀ impl,
+(∀ s, problem_spec impl s) ↔
+(∀ s, generated_spec impl s) :=
+-- end_def spec_isomorphism
+-- start_def spec_isomorphism_proof
+sorry
+-- end_def spec_isomorphism_proof
+
+
+-- start_def implementation_signature
+def implementation (s: String) : Int := sorry
+-- end_def implementation_signature
+
+-- start_def implementation
+-- end_def implementation
+
+-- start_def test_cases
+-- #test implementation "aBCdEf" = 1
+-- #test implementation "abcdefg" = 0
+-- #test implementation "dBBE" = 0
+-- end_def test_cases
+
+
+-- start_def correctness_definition
+theorem correctness
+(s: String)
+: problem_spec implementation s
+:=
+-- end_def correctness_definition
+-- start_def correctness_proof
+by
+sorry
+-- end_def correctness_proof
