src/lean4/human_eval/problem_99.lean
@@ -1,0 +1,95 @@
+import Imports.AllImports
+import Std
+-- start_def problem_details
+/--
+function_signature: "def closest_integer(s : String) -> Option Int"
+docstring: |
+    Create a function that takes a value (string) representing a number
+    and returns the closest integer to it. If the number is equidistant
+    from two integers, round it away from zero.
+test_cases:
+  - input: "10"
+    expected_output: 10
+  - input: "15.3"
+    expected_output: 15
+-/
+-- end_def problem_details
+
+-- start_def problem_spec
+def problem_spec
+-- function signature
+(implementation: String → Option Int)
+-- inputs
+(s: String) :=
+-- spec
+let numeric_characters := ["-", "0", "1", "2", "3", "4", "5", "6", "7", "8", "9", "."]
+let is_valid_string :=
+  s.length > 0 ∧
+  s.count (".".get! 0) ≤ 1 ∧
+  s.count ("-".get! 0) ≤ 1 ∧
+  s.data.all (fun c => numeric_characters.contains (String.mk [c])) ∧
+  (s.count ("-".get! 0) = 1 → s.data.head! = '-')
+
+let spec (result : Option Int) := match result with
+  | some result =>
+    is_valid_string ∧
+    let parts := s.split (fun c => c = '.')
+    (parts.length = 1 → result = s.toInt!) ∧
+    (parts.length = 2 →
+      let integer_part := parts.get! 0
+      let is_negative := s.data.head! = '-'
+      |((integer_part.toInt! - result) : ℚ)| ≤ 0.5 ∧
+      (is_negative → |((integer_part.toInt! - result) : ℚ)| = 0.5 → integer_part.toInt? < result) ∧
+      (¬is_negative → |((integer_part.toInt! - result) : ℚ)| = 0.5 → integer_part.toInt? > result)
+    )
+  | none => ¬ is_valid_string
+-- program termination
+∃ result,
+  implementation s = result ∧
+  spec result
+
+-- start_def generated_spec
+def generated_spec
+-- function signature
+(impl: String → Option Int)
+-- inputs
+(s: String) : Prop :=
+--end_def generated_spec
+--start_def generated_spec_body
+sorry
+--end_def generated_spec_body
+
+-- start_def spec_isomorphism
+theorem spec_isomorphism:
+∀ impl,
+(∀ s, problem_spec impl s) ↔
+(∀ s, generated_spec impl s) :=
+-- end_def spec_isomorphism
+-- start_def spec_isomorphism_proof
+sorry
+-- end_def spec_isomorphism_proof
+
+
+-- start_def implementation_signature
+def implementation (s: String) : Option Int := sorry
+-- end_def implementation_signature
+
+-- start_def implementation
+-- end_def implementation
+
+-- start_def test_cases
+-- #test implementation "10" = some 10
+-- #test implementation "15.3" = some 15
+-- end_def test_cases
+
+
+-- start_def correctness_definition
+theorem correctness
+(s: String)
+: problem_spec implementation s
+:=
+-- end_def correctness_definition
+-- start_def correctness_proof
+by
+sorry
+-- end_def correctness_proof
